fstar/MLS.TreeSync.ExternalPath.fst
@@ -13,48 +13,59 @@ open MLS.Result
 
 #set-options "--fuel 1 --ifuel 1"
 
-//TODO: this function has bad complexity (because some subtrees are converted a lot of time)
-//Do we care?
-val external_pathsync_to_pathsync_aux: #bytes:Type0 -> {|crypto_bytes bytes|} -> #l:nat -> #n:tree_size l -> #i:leaf_index n -> option (sign_private_key bytes & sign_nonce bytes) -> bytes -> nat -> treesync bytes l n -> external_pathsync bytes l n i -> result (pathsync bytes l n i)
-let rec external_pathsync_to_pathsync_aux #bytes #cb #l #n #i opt_sign_key parent_parent_hash nb_left_leaves t p =
+val sign_leaf: #bytes:Type0 -> {|crypto_bytes bytes|} -> sign_private_key bytes -> sign_nonce bytes -> leaf_package_t bytes -> bytes -> bytes -> result (leaf_package_t bytes)
+let sign_leaf #bytes #cb sign_key entropy lp parent_parent_hash group_id =
+  if not (length parent_parent_hash < 256) then
+    internal_failure "sign_leaf: parent hash too long"
+  else if not (lp.source = LNS_commit ()) then
+    error "sign_leaf: source is not a commit"
+  else (
+    let lp = ({lp with parent_hash = parent_parent_hash} <: leaf_package_t bytes) in
+    ln <-- leaf_package_to_network lp;
+    if not (ln.data.source = LNS_commit ()) then
+      internal_failure "sign_leaf: source is not a commit (???)"
+    else if not (length group_id < 256) then
+      internal_failure "sign_leaf: group_id is too long"
+    else (
+      let ln_tbs = {
+        data = ln.data;
+        group_id = group_id;
+      } in
+      let tbs_bytes = serialize (leaf_node_tbs_nt bytes) ln_tbs in
+      new_signature <-- sign_with_label sign_key (string_to_bytes #bytes "LeafNodeTBS") tbs_bytes entropy;
+      return ({lp with signature = new_signature} <: leaf_package_t bytes)
+    )
+  )
+
+val external_pathsync_to_pathsync_aux: #bytes:Type0 -> {|crypto_bytes bytes|} -> #l:nat -> #n:tree_size l -> #i:leaf_index n -> option (sign_private_key bytes & sign_nonce bytes) -> bytes -> nat -> treesync bytes l n -> external_pathsync bytes l n i -> bytes -> result (pathsync bytes l n i)
+let rec external_pathsync_to_pathsync_aux #bytes #cb #l #n #i opt_sign_key parent_parent_hash nb_left_leaves t p group_id =
   match t, p with
   | _, PLeaf lp ->
     lp <-- (
       match opt_sign_key with
       | None -> return lp
       | Some (sign_key, entropy) -> (
-        if not (length parent_parent_hash < 256) then
-          internal_failure "external_pathsync_to_pathsync_aux: parent hash too long"
-        else (
-          new_extensions <-- set_parent_hash_extension lp.extensions ({parent_hash = parent_parent_hash});
-          let lp = ({lp with extensions = new_extensions}) in
-          key_package <-- treesync_to_keypackage lp;
-          let leaf_package_bytes = serialize (key_package_tbs_nt bytes) key_package.tbs in
-          new_signature <-- sign_with_label sign_key (string_to_bytes #bytes "KeyPackageTBS") leaf_package_bytes entropy;
-          return ({lp with signature = new_signature} <: leaf_package_t bytes)
-        )
+        sign_leaf sign_key entropy lp parent_parent_hash group_id
       )
     );
-    leaf_errors <-- check_leaf 0 (Some lp); //TODO hack: we know that the leaf index is only used for the errors, so we can set it to 0
-    let parent_hash_ext = get_parent_hash_extension lp.extensions in
-    //TODO: hack while openmls' test vectors are broken
-    if not (IE_Good? leaf_errors || (match leaf_errors with |IE_Errors [IE_LeafError LIE_ExtensionsNotInCapabilities _] -> true |IE_Errors [IE_LeafError LIE_NoCapabilities _] -> true| _ -> false)) then
+    leaf_errors <-- check_leaf 0 (Some lp) group_id; //TODO hack: we know that the leaf index is only used for the errors, so we can set it to 0
+    if not (IE_Good? leaf_errors) then
       error "external_pathsync_to_pathsync_aux: invalid leaf"
-    else if not (Some? parent_hash_ext) then
-      error "external_pathsync_to_pathsync_aux: leaf don't contain any parent hash"
-    else if not ((Some?.v parent_hash_ext).parent_hash = parent_parent_hash) then
+    else if not (lp.source = LNS_commit ()) then
+      error "external_pathsync_to_pathsync_aux: leaf source isn't commit"
+    else if not ((lp.parent_hash <: bytes) = parent_parent_hash) then
       error "external_pathsync_to_pathsync_aux: leaf contain an invalid parent hash"
     else
       return (PLeaf (Some lp))
   | TSkip _ t', PSkip _ p' ->
-    result <-- external_pathsync_to_pathsync_aux opt_sign_key parent_parent_hash nb_left_leaves t' p';
+    result <-- external_pathsync_to_pathsync_aux opt_sign_key parent_parent_hash nb_left_leaves t' p' group_id;
     return (PSkip _ result)
   | TNode _ left right, PNode np p_next ->
     let (|dir, next_i|) = child_index l i in
     let (child, sibling) = order_subtrees dir (left, right) in
     let child_nb_left_leaves = if dir = Left then nb_left_leaves else nb_left_leaves + (pow2 (l-1)) in
     parent_hash <-- compute_parent_hash_from_dir np.content parent_parent_hash nb_left_leaves t dir;
-    result_p_next <-- external_pathsync_to_pathsync_aux opt_sign_key parent_hash child_nb_left_leaves child p_next;
+    result_p_next <-- external_pathsync_to_pathsync_aux opt_sign_key parent_hash child_nb_left_leaves child p_next group_id;
     return (PNode (Some ({
       version = 0;
       unmerged_leaves = [];
@@ -62,7 +73,7 @@ let rec external_pathsync_to_pathsync_aux #bytes #cb #l #n #i opt_sign_key paren
       content = np;
     } <: node_package_t bytes)) result_p_next)
 
-val external_pathsync_to_pathsync: #bytes:Type0 -> {|crypto_bytes bytes|} -> #l:nat -> #n:tree_size l -> #i:leaf_index n -> option (sign_private_key bytes & sign_nonce bytes) -> treesync bytes l n -> external_pathsync bytes l n i -> result (pathsync bytes l n i)
-let external_pathsync_to_pathsync #bytes #cb #l #n #i opt_sign_key t p =
-  external_pathsync_to_pathsync_aux opt_sign_key empty 0 t p
+val external_pathsync_to_pathsync: #bytes:Type0 -> {|crypto_bytes bytes|} -> #l:nat -> #n:tree_size l -> #i:leaf_index n -> option (sign_private_key bytes & sign_nonce bytes) -> treesync bytes l n -> external_pathsync bytes l n i -> bytes -> result (pathsync bytes l n i)
+let external_pathsync_to_pathsync #bytes #cb #l #n #i opt_sign_key t p group_id =
+  external_pathsync_to_pathsync_aux opt_sign_key empty 0 t p group_id
 
