fstar/MLS.TreeSync.KeyPackageRef.fst
@@ -9,22 +9,27 @@ open MLS.NetworkBinder
 open MLS.Crypto
 open MLS.Result
 
-val leaf_package_to_kp_ref: #bytes:Type0 -> {|crypto_bytes bytes|} -> leaf_package_t bytes -> result (key_package_ref_nt bytes)
-let leaf_package_to_kp_ref #bytes #cb lp =
-  kp <-- treesync_to_keypackage lp;
+val compute_key_package_ref: #bytes:Type0 -> {|crypto_bytes bytes|} -> key_package_nt bytes -> result (key_package_ref_nt bytes)
+let compute_key_package_ref #bytes #cb kp =
   let kp_bytes: bytes = serialize (key_package_nt bytes) kp in
   make_keypackage_ref kp_bytes
 
-val key_package_ref_to_index: #bytes:Type0 -> {|crypto_bytes bytes|} -> #l:nat -> #n:tree_size l -> treesync bytes l n -> key_package_ref_nt bytes -> result (option (leaf_index n))
-let key_package_ref_to_index #bytes #cb #l #n t kp_ref =
+val compute_leaf_node_ref: #bytes:Type0 -> {|crypto_bytes bytes|} -> leaf_package_t bytes -> result (leaf_node_ref_nt bytes)
+let compute_leaf_node_ref #bytes #cb lp =
+  leaf <-- leaf_package_to_network lp;
+  let leaf_bytes: bytes = serialize (leaf_node_nt bytes) leaf in
+  make_leafnode_ref leaf_bytes
+
+val leaf_node_ref_to_index: #bytes:Type0 -> {|crypto_bytes bytes|} -> #l:nat -> #n:tree_size l -> treesync bytes l n -> leaf_node_ref_nt bytes -> result (option (leaf_index n))
+let leaf_node_ref_to_index #bytes #cb #l #n t ln_ref =
   let leaves = get_leaf_list t in
-  kp_refs <-- mapM (fun olp ->
+  ln_refs <-- mapM (fun olp ->
     match olp with
     | Some lp -> (
-        kp_ref <-- leaf_package_to_kp_ref lp;
+        kp_ref <-- compute_leaf_node_ref #bytes #cb lp;
         return (Some kp_ref)
     )
     | None -> return None
   ) leaves;
-  let opt_res = (find_first (fun x -> x = Some kp_ref) kp_refs) in
+  let opt_res = (find_first (fun x -> x = Some ln_ref) ln_refs) in
   return #(option (leaf_index n)) opt_res
